src/tls/FFI.fst
@@ -70,7 +70,7 @@ private let errno description txt : ML int =
     | None    -> "(None)" in (
   trace ("returning error: "^txt0^" "^txt^"\n"); (
   match description with
-  | Some ad -> FStar.UInt8.v (snd (cbyte2 (Alert.alertBytes ad)))
+  | Some ad ->  let _, e = split (Alert.alertBytes ad) 2 in int_of_bytes e
   | None    -> -1 ))
 
 
