src/tls/Parse.fst
@@ -227,12 +227,12 @@ type ffdhe =
   | FFDHE6144
   | FFDHE8192
 
-type unknownNG = u:(U8.t * U8.t){
- (let (b1,b2) = (U8.v (fst u), U8.v (snd u)) in
-    (b1 = 0 ==> b2 <> 0x17 /\ b2 <> 0x18 /\ b2 <> 0x19
-                 /\ b2 <> 0x1d /\ b2 <> 0x1e) /\
-    (b1 = 1 ==> b2 <> 0x00 /\ b2 <> 0x01 /\ b2 <> 0x02
-                 /\ b2 <> 0x03 /\ b2 <> 0x04))}
+type unknownNG = u:(byte * byte){
+    (let b1, b2 = u in
+    (b1 = 0z ==> b2 <> 0x17z /\ b2 <> 0x18z /\ b2 <> 0x19z
+                 /\ b2 <> 0x1dz /\ b2 <> 0x1ez) /\
+    (b1 = 1z ==> b2 <> 0x00z /\ b2 <> 0x01z /\ b2 <> 0x02z
+                 /\ b2 <> 0x03z /\ b2 <> 0x04z))}
 
 (** TLS 1.3 named groups for (EC)DHE key exchanges *)
 type namedGroup =
@@ -271,9 +271,8 @@ let namedGroupBytes ng =
     end
   | NG_UNKNOWN u	-> abyte2 u
 
-(* TODO: move to Platform.Bytes *)
 let abyte2_inj x1 x2 : Lemma
-  (abyte2 x1 == abyte2 x2 ==> U8.v (fst x1) = U8.v (fst x2) /\ U8.v (snd x1) = U8.v (snd x2))
+  (abyte2 x1 == abyte2 x2 ==> fst x1 = fst x2 /\ snd x1 = snd x2)
   [SMTPat (abyte2 x1); SMTPat (abyte2 x2)]
 = let s1 = abyte2 x1 in
   let s2 = abyte2 x2 in
